ast: Add children to Expr.Unsupported constructor
These are normally ignored, but included in Depth calculations to make
it possible to prove termination of code that looks at them.

src/Tools/Auditor/Auditor.dfy
@@ -21,7 +21,17 @@ module {:extern "Bootstrap.Tools.Auditor"} {:options "-functionSyntax:4"} Bootst
 
   //// AST traversals ////
 
-  predicate IsAssumeStatement(e: Expr) {
+  function {:opaque} Any<T>(P: T ~> bool, ts: seq<T>) : (b: bool)
+    reads P.reads
+    requires forall t | t in ts :: P.requires(t)
+    ensures b == exists t | t in ts :: P(t)
+    ensures b == exists i | 0 <= i < |ts| :: P(ts[i])
+  {
+    !Seq.All(x reads P.reads requires P.requires(x) => !P(x), ts)
+  }
+
+  predicate IsAssumeStatement(e: Expr)
+  {
     && e.Apply?
     && e.aop.Eager?
     && e.aop.eOp.Builtin?
@@ -29,8 +39,12 @@ module {:extern "Bootstrap.Tools.Auditor"} {:options "-functionSyntax:4"} Bootst
     && e.aop.eOp.builtin.predTy.Assume?
   }
 
-  predicate ContainsAssumeStatement(e: Expr) {
-    Deep.Any_Expr(e, IsAssumeStatement)
+  predicate ContainsAssumeStatement(e: Expr)
+    decreases e.Depth()
+  {
+    || Deep.Any_Expr(e, (c:Expr) => IsAssumeStatement(c))
+    || (&& e.Unsupported?
+        && Any((c:Expr) requires c.Depth() < e.Depth() => ContainsAssumeStatement(c), e.children))
   }
 
   //// Tag extraction and processing ////
