src/AST/Syntax.dfy
@@ -259,7 +259,7 @@ module Exprs {
     | Block(stmts: seq<Expr>)
     | Bind(vars: seq<string>, vals: seq<Expr>, body: Expr)
     | If(cond: Expr, thn: Expr, els: Expr) // DISCUSS: Lazy op node?
-    | Unsupported(description: string)
+    | Unsupported(description: string, children: seq<Expr>)
   {
     function method Depth() : nat {
       1 + match this {
@@ -280,8 +280,11 @@ module Exprs {
           )
         case If(cond, thn, els) =>
           Math.Max(cond.Depth(), Math.Max(thn.Depth(), els.Depth()))
-        case Unsupported(_) =>
-          0
+        // We ignore the children of Unsupported nodes for normal
+        // traversals, but when we do want to look at the children
+        // it's useful to be able to prove termination.
+        case Unsupported(_, args) =>
+          Seq.MaxF(var f := (e: Expr) requires e in args => e.Depth(); f, args, 0)
       }
     }
 
@@ -296,7 +299,8 @@ module Exprs {
         case Block(exprs) => exprs
         case Bind(vars, vals, body) => vals + [body]
         case If(cond, thn, els) => [cond, thn, els]
-        case Unsupported(_) => []
+        // We ignore the children for normal traversals
+        case Unsupported(_, children) => []
       }
     }
   }
@@ -337,7 +341,7 @@ module Exprs {
         e'.If?
       case Bind(vars, vals, body) =>
         e'.Bind? && |vars| == |e'.vars| && |vals| == |e'.vals|
-      case Unsupported(description) =>
+      case Unsupported(description, _) =>
         e'.Unsupported? && e'.description == description
     }
   }
